theory/bpfConsistencyAux1.thy
@@ -3,6 +3,101 @@ theory bpfConsistencyAux1
   x64Assembler x64DecodeProof Mem JITCommType
 begin
 
+lemma push_pop_subgoal_rr_aux2_1:
+  assumes a0:"xins = [Ppushl_r x64Syntax.RCX, Ppopl x64Syntax.RCX]" and 
+    a1:"Next reg' m' = (exec_instr (xins!0) 1 reg m) " and
+    a2:"Next reg'' m'' = (exec_instr (xins!1) 1 reg' m') "
+  shows "reg'' (IR x64Syntax.RCX) = reg (IR x64Syntax.RCX)"
+proof -
+  have b0:"Next reg' m' = exec_push 1 M32 m reg (reg (IR x64Syntax.RCX))" using exec_instr_def by (simp add: a0 a1)
+  have b1:"Next reg' m' =
+    (case storev M32 m (sub64 (reg (IR SP)) (vlong_of_memory_chunk M32)) (reg (IR ireg.RCX)) of None \<Rightarrow> Stuck
+     | Some (x::64 word \<Rightarrow> 8 word option option) \<Rightarrow>
+         Next
+          ((undef_regs [CR ZF, CR CF, CR PF, CR SF, CR OF] (reg(IR SP := sub64 (reg (IR SP)) (vlong_of_memory_chunk M32))))
+           (RIP := add64 (undef_regs [CR ZF, CR CF, CR PF, CR SF, CR OF] (reg(IR SP := sub64 (reg (IR SP)) (vlong_of_memory_chunk M32))) RIP) (Vlong ((1::64 word) + (1::64 word)))))
+          x) " using b0 nextinstr_nf_def nextinstr_def exec_push_def by metis
+  have b2_1:"(exec_instr (xins!0) 1 reg m) = Next reg' m' \<longrightarrow> storev M32 m (sub64 (reg (IR SP)) (vlong_of_memory_chunk M32)) (reg (IR ireg.RCX)) \<noteq> None" using push_pop_subgoal_rr_aux1 a0 a1 
+    by (metis b1 option.case(1) outcome.simps(3))
+  have b2_2:"storev M32 m (sub64 (reg (IR SP)) (vlong_of_memory_chunk M32)) (reg (IR ireg.RCX)) \<noteq> None" using b2_1 a1 by simp
+  have b2:"storev M32 m (sub64 (reg (IR SP)) (vlong_of_memory_chunk M32)) (reg (IR ireg.RCX))= Some m'" using b1 b2_2 by auto
+  have b3:"reg' (IR SP) = sub64 (reg (IR SP)) (vlong_of_memory_chunk M32)" using b1 b2 by auto
+  let "?sp" = "reg' (IR SP)"
+  have b4:"storev M32 m (reg' (IR SP)) (reg (IR ireg.RCX)) = Some m'" using b2 b3 by simp
+  have c0:"Next reg'' m'' = exec_pop (1::64 word) M32 m' reg' (IR ireg.RCX)" using exec_instr_def by (simp add: a0 a2)
+  have c2:"loadv M32 m' (reg' (IR SP)) = Some (reg (IR ireg.RCX))" using b4 store_load_consistency by simp
+  let "?v" = " (reg (IR ireg.RCX))"
+  have c3:" Next reg'' m'' =
+    (case loadv M32 m' (reg' (IR SP)) of None \<Rightarrow> Stuck
+     | Some (v::val) \<Rightarrow>
+         Next
+          ((undef_regs [CR ZF, CR CF, CR PF, CR SF, CR OF] (reg'(IR ireg.RCX := ?v, IR SP := add64 (reg' (IR SP)) (vlong_of_memory_chunk M32))))
+           (RIP := add64 (undef_regs [CR ZF, CR CF, CR PF, CR SF, CR OF] (reg'(IR ireg.RCX := ?v, IR SP := add64 (reg' (IR SP)) (vlong_of_memory_chunk M32))) RIP) (Vlong ((1::64 word) + (1::64 word)))))
+          m')" using nextinstr_nf_def nextinstr_def exec_pop_def c2 
+    using c0 by force
+  have c4:"reg''(IR ireg.RCX) = ?v" using exec_pop_def c2 c3 by auto
+  thus ?thesis using c4 by simp
+qed
+
+lemma push_pop_subgoal_rr_aux2_2:
+  assumes a0:"xins = [Ppushl_r x64Syntax.RCX, Ppopl x64Syntax.RCX]" and 
+    a1:"Next reg'' m'' = interp3 xins (Next reg m)" 
+  shows "reg'' (IR x64Syntax.RCX) = reg (IR x64Syntax.RCX)"
+proof-
+  have b0:"length xins = (2::nat)" using a0 by simp
+  thus ?thesis using b0 a0 a1 push_pop_subgoal_rr_aux2_1 interp3_length2_aux2
+    by metis
+qed
+
+lemma push_pop_subgoal_rr_aux2_3:
+  assumes a0:"hd xins = Ppushl_r x64Syntax.RCX" and 
+          a1:"last xins = Ppopl x64Syntax.RCX"and
+          a2:"interp3 (butlast(tl xins)) (Next reg' m') = Next reg2 m'"and
+          a3:"Next reg'' m'' = (exec_instr (last xins) 1 reg2 m') " and
+          a5:"Next reg' m' = (exec_instr (xins!0) 1 reg m) " and
+          a6:"reg' (IR SP) =  reg2 (IR SP)"
+  shows "reg'' (IR x64Syntax.RCX) = reg (IR x64Syntax.RCX)"
+proof-
+  let ?midlist = "butlast(tl xins)"
+  have b0_1:"xins = [Ppushl_r x64Syntax.RCX]@?midlist@[Ppopl x64Syntax.RCX]" using a0 a1
+    by (metis append_Cons append_Nil append_butlast_last_id hd_Nil_eq_last instruction.distinct(5787) last_ConsL last_tl list.collapse)
+  have b0:"Next reg' m' = exec_push 1 M32 m reg (reg (IR x64Syntax.RCX))" using exec_instr_def a0 
+    using exec_push_def a5 a0 
+    by (smt (z3) a1 hd_Nil_eq_last hd_conv_nth instruction.distinct(5787) instruction.simps(6295))
+  have b1:"Next reg' m' =
+    (case storev M32 m (sub64 (reg (IR SP)) (vlong_of_memory_chunk M32)) (reg (IR ireg.RCX)) of None \<Rightarrow> Stuck
+     | Some (x::64 word \<Rightarrow> 8 word option option) \<Rightarrow>
+         Next
+          ((undef_regs [CR ZF, CR CF, CR PF, CR SF, CR OF] (reg(IR SP := sub64 (reg (IR SP)) (vlong_of_memory_chunk M32))))
+           (RIP := add64 (undef_regs [CR ZF, CR CF, CR PF, CR SF, CR OF] (reg(IR SP := sub64 (reg (IR SP)) (vlong_of_memory_chunk M32))) RIP) (Vlong ((1::64 word) + (1::64 word)))))
+          x) " using b0 nextinstr_nf_def nextinstr_def exec_push_def by metis
+  have b2_1:"(exec_instr (xins!0) 1 reg m) = Next reg' m' \<longrightarrow> storev M32 m (sub64 (reg (IR SP)) (vlong_of_memory_chunk M32)) (reg (IR ireg.RCX)) \<noteq> None" using push_pop_subgoal_rr_aux1 a0 a1 
+    by (metis b1 option.case(1) outcome.simps(3))
+  have b2_2:"storev M32 m (sub64 (reg (IR SP)) (vlong_of_memory_chunk M32)) (reg (IR ireg.RCX)) \<noteq> None" using b2_1 a5 by simp
+  have b2:"storev M32 m (sub64 (reg (IR SP)) (vlong_of_memory_chunk M32)) (reg (IR ireg.RCX))= Some m'" using b1 b2_2 by auto
+  have b3:"reg' (IR SP) = sub64 (reg (IR SP)) (vlong_of_memory_chunk M32)" using b1 b2 by auto
+  let "?sp" = "reg' (IR SP)"
+  have b4:"storev M32 m (reg' (IR SP)) (reg (IR ireg.RCX)) = Some m'" using b2 b3 by simp
+  have b5:"interp3 (butlast(xins)) (Next reg m) = Next reg2 m'" using a2 a5 b0_1 a0
+    by (metis append_Cons append_Nil butlast.simps(1) butlast.simps(2) interp3.simps(2) list.sel(3) list.simps(3) nth_Cons_0 outcome.case(1))
+  have b6:"(exec_instr (last xins) 1 reg2 m') = Next reg'' m''" using a5 a1 a2 a3 b5 by simp
+  have c0:"Next reg'' m'' = exec_pop (1::64 word) M32 m' reg2 (IR ireg.RCX)" using exec_instr_def using b6 a1 by simp
+  have c1:"loadv M32 m' (reg' (IR SP)) = Some (reg (IR ireg.RCX))" using b4 store_load_consistency by simp
+  have c2:"loadv M32 m' (reg2 (IR SP)) = Some (reg (IR ireg.RCX))" using b4 c1 a6 by simp
+  let "?v" = " (reg (IR ireg.RCX))"
+  have c3:" Next reg'' m'' =
+    (case loadv M32 m' (reg2 (IR SP)) of None \<Rightarrow> Stuck
+     | Some (v::val) \<Rightarrow>
+         Next
+          ((undef_regs [CR ZF, CR CF, CR PF, CR SF, CR OF] (reg2(IR ireg.RCX := ?v, IR SP := add64 (reg2 (IR SP)) (vlong_of_memory_chunk M32))))
+           (RIP := add64 (undef_regs [CR ZF, CR CF, CR PF, CR SF, CR OF] (reg2(IR ireg.RCX := ?v, IR SP := add64 (reg2 (IR SP)) (vlong_of_memory_chunk M32))) RIP) (Vlong ((1::64 word) + (1::64 word)))))
+          m')" using nextinstr_nf_def nextinstr_def exec_pop_def 
+    using c0 c2 by simp
+  have c4:"reg''(IR ireg.RCX) = ?v" using exec_pop_def c2 c3 by simp
+  thus ?thesis using c4 by simp
+qed
+
+
 lemma div_subgoal_rr_aux1:"
     bins = BPF_ALU64 BPF_DIV dst (SOReg src) \<Longrightarrow> (BPF_OK pc rs' m' ss' is_v1 (cur_cu+1) remain_cu) = step fuel bins rs m ss is_v1 cur_cu remain_cu \<Longrightarrow>
     \<forall> r \<noteq> dst. rs' r = rs r"
@@ -14,7 +109,7 @@ lemma div_subgoal_rr_aux1:"
   done
 
 
-lemma div_subgoal_rr_aux3_1:
+lemma div_subgoal_rr_aux3:
   assumes a0:"bins = BPF_ALU64 BPF_DIV dst (SOReg src)" and
      a1:"xins = [Ppushl_r x64Syntax.RCX, Pmovq_rr (x64Syntax.RCX) ri,Pshlq_r rd,Ppopl x64Syntax.RCX]" and
      a2:"(BPF_OK pc rs' m' ss' is_v1 (cur_cu+1) remain_cu) = step fuel bins rs m ss is_v1 cur_cu remain_cu" and
@@ -30,7 +125,7 @@ lemma div_subgoal_rr_aux3_1:
   sorry
 
 
-lemma div_subgoal_rr_aux3:
+(*lemma div_subgoal_rr_aux3_1:
   assumes a0:"bins = BPF_ALU64 BPF_DIV dst (SOReg src)" and
      a1:"xins = Pdivq_r ri" and
      a2:"(BPF_OK pc rs' m' ss' is_v1 (cur_cu+1) remain_cu) = step fuel bins rs m ss is_v1 cur_cu remain_cu" and
@@ -45,7 +140,93 @@ lemma div_subgoal_rr_aux3:
      a11:"reg (IR x64Syntax.RAX) = Vlong 0"
      shows "Vlong (rs' dst) = reg' (IR (bpf_to_x64_reg dst))"
   sorry
-  
+*)
+
+(*value" divmod64u (Vlong 0) (Vlong 4) (Vlong 3)"
+
+lemma "xins = Pdivq_r ri \<Longrightarrow> result = exec_instr xins sz reg m \<Longrightarrow> 
+  reg (IR x64Syntax.RAX) = Vlong n2 \<Longrightarrow> reg (IR x64Syntax.RDX) = Vlong 0 \<Longrightarrow> reg (IR ri) = Vlong n1 \<Longrightarrow> 
+  (ucast(n1+n2)::128 word) \<le> ucast u64_MAX \<Longrightarrow> result \<noteq> Stuck"
+  apply(unfold exec_instr_def)
+  apply(cases "xins",simp_all)
+  apply(unfold eval_alu64_def eval_alu64_aux1_def divmod64u_def Let_def,simp_all)
+  done
+*)
+
+lemma ucast_for_div:"(x::u64) div (y::u64) = ucast(((ucast x)::u128) div ((ucast y)::u128))"
+  sorry
+
+lemma div_subgoal_rr_aux3_1:
+    "bins = BPF_ALU64 BPF_DIV dst (SOReg src) \<Longrightarrow> 
+    xins = Pdivq_r ri \<Longrightarrow>
+    (BPF_OK pc rs' m' ss' is_v1 (cur_cu+1) remain_cu) = step fuel bins rs m ss is_v1 cur_cu remain_cu \<Longrightarrow> 
+    Next reg' m' = exec_instr xins sz reg m \<Longrightarrow>
+    x64Syntax.RAX = (bpf_to_x64_reg dst) \<Longrightarrow> 
+    ri = (bpf_to_x64_reg src) \<Longrightarrow> 
+    reg (IR x64Syntax.RAX) = Vlong n1 \<Longrightarrow> 
+    reg (IR ri) = Vlong n2 \<Longrightarrow> 
+    n1 = rs dst \<Longrightarrow> 
+    n2  = rs src \<Longrightarrow> 
+    n2 \<noteq> 0 \<Longrightarrow> 
+    reg (IR x64Syntax.RDX) = Vlong 0 \<Longrightarrow>
+    Vlong (rs' dst) = reg' (IR (bpf_to_x64_reg dst))"
+(*(ucast(n1+n2)::128 word) \<le> ucast u64_MAX \<Longrightarrow>*)
+  apply(unfold exec_instr_def)
+  apply(cases xins, simp_all)
+  subgoal for x31a apply(cases "is_v1",simp_all)
+     apply(unfold eval_alu64_def eval_alu64_aux1_def Let_def eval_reg_def,simp_all)
+    apply(unfold divmod64u_def Let_def, simp_all)
+    apply(simp add:nextinstr_nf_def nextinstr_def add64_def )
+    apply(cases "reg RIP",simp_all)
+    using ucast_for_div apply blast
+    subgoal for x2 using ucast_for_div apply blast
+      done
+    subgoal for x3 using ucast_for_div apply blast
+      done
+    subgoal for x4 using ucast_for_div apply blast
+      done
+    subgoal for x5 using ucast_for_div apply blast
+      done
+  done
+  done
+
+lemma div_subgoal_rr_aux3_2:
+    "bins = BPF_ALU64 BPF_DIV dst (SOReg src) \<Longrightarrow> 
+    xins = Pdivq_r ri \<Longrightarrow>
+    (BPF_OK pc rs' m' ss' is_v1 (cur_cu+1) remain_cu) = step fuel bins rs m ss is_v1 cur_cu remain_cu \<Longrightarrow> 
+    Next reg' m' = exec_instr xins sz reg m \<Longrightarrow>
+    x64Syntax.RAX = (bpf_to_x64_reg dst) \<Longrightarrow> 
+    ri = (bpf_to_x64_reg src) \<Longrightarrow> 
+    reg (IR x64Syntax.RAX) = Vlong n1 \<Longrightarrow> 
+    reg (IR ri) = Vlong n2 \<Longrightarrow> 
+    n1 = rs dst \<Longrightarrow> 
+    n2  = rs src \<Longrightarrow> 
+    n2 = 0 \<Longrightarrow> 
+    reg (IR x64Syntax.RDX) = Vlong 0 \<Longrightarrow>
+    Vlong (rs' dst) = reg' (IR (bpf_to_x64_reg dst))"
+(*(ucast(n1+n2)::128 word) \<le> ucast u64_MAX \<Longrightarrow>*)
+  apply(unfold exec_instr_def)
+  apply(cases xins, simp_all)
+  subgoal for x31a apply(cases "is_v1",simp_all)
+     apply(unfold eval_alu64_def eval_alu64_aux1_def Let_def eval_reg_def,simp_all)
+    done
+  done
+
+lemma div_subgoal_rr_aux3_3:
+    "bins = BPF_ALU64 BPF_DIV dst (SOReg src) \<Longrightarrow> 
+    xins = Pdivq_r ri \<Longrightarrow>
+    (BPF_OK pc rs' m' ss' is_v1 (cur_cu+1) remain_cu) = step fuel bins rs m ss is_v1 cur_cu remain_cu \<Longrightarrow> 
+    Next reg' m' = exec_instr xins sz reg m \<Longrightarrow>
+    x64Syntax.RAX = (bpf_to_x64_reg dst) \<Longrightarrow> 
+    ri = (bpf_to_x64_reg src) \<Longrightarrow> 
+    reg (IR x64Syntax.RAX) = Vlong n1 \<Longrightarrow> 
+    reg (IR ri) = Vlong n2 \<Longrightarrow> 
+    n1 = rs dst \<Longrightarrow> 
+    n2  = rs src \<Longrightarrow> 
+    reg (IR x64Syntax.RDX) = Vlong 0 \<Longrightarrow>
+    Vlong (rs' dst) = reg' (IR (bpf_to_x64_reg dst))"
+(*(ucast(n1+n2)::128 word) \<le> ucast u64_MAX \<Longrightarrow>*)
+  using div_subgoal_rr_aux3_1 div_subgoal_rr_aux3_2 by metis
 
 lemma reg_rax_rdx1:"(bpf_to_x64_reg dst) = x64Syntax.RAX \<longrightarrow> (bpf_to_x64_reg dst) \<noteq> x64Syntax.RDX" 
   apply(cases dst) 
@@ -72,12 +253,14 @@ proof -
     using a8 calculation by presburger
     moreover have b1:"Vlong (rs dst) = reg (IR (bpf_to_x64_reg dst))" using a6 spec by simp
     moreover have b2:"Vlong (rs src) = reg (IR (bpf_to_x64_reg src))" using a6 spec by simp
-    hence b3:"Vlong (rs' dst) = reg' (IR (bpf_to_x64_reg dst))" using div_subgoal_rr_aux1 b0 b1 b2 a0 a4 a5 a7 sorry
+    hence b3:"Vlong (rs' dst) = reg' (IR (bpf_to_x64_reg dst))" using div_subgoal_rr_aux1 b0 b1 b2 a0 a4 a5 a7 div_subgoal_rr_aux3_3 sorry
     have b4:"\<forall> r \<noteq> dst. reg'(IR (bpf_to_x64_reg r)) = reg (IR (bpf_to_x64_reg r))" using b0 a5 sorry
     have b5:"\<forall> r \<noteq> dst. Vlong (rs' r) = Vlong (rs r)" using a0 a4 div_subgoal_rr_aux1 by blast
     have b6:"\<forall> r \<noteq> dst. Vlong (rs r) = reg (IR (bpf_to_x64_reg r))" using a6 by blast
     have b7:"(\<forall> r \<noteq> dst. Vlong (rs' r) = reg' (IR (bpf_to_x64_reg r)))" by(simp add:b4 b5 b6) 
     thus ?thesis using b3 by fastforce
   qed
+
+
 
 end
